destr_list

tests/layeff/LowParseWriters.Parsers.fst
@@ -81,3 +81,184 @@ let valid_synth_parse_vldata
     ()
   );
 }
+
+noeq
+type rlptr = {
+  rlptr_base: B.buffer u8;
+  rlptr_len: (rlptr_len: U32.t { rlptr_len == B.len rlptr_base });
+}
+
+let valid_rlptr
+  p inv x
+=
+  let base = x.rlptr_base in
+  let len = B.len base in
+  let sl = LP.make_slice base len in
+  LP.valid_list (get_parser p) inv.h0 sl 0ul len /\
+  inv.lread `B.loc_includes` B.loc_buffer base
+
+let deref_list_spec
+  #p #inv x
+=
+  let base = x.rlptr_base in
+  let len = B.len base in
+  let sl = LP.make_slice base len in
+  LP.contents_list (get_parser p) inv.h0 sl 0ul len
+
+let valid_rlptr_frame
+  #p #inv x inv'
+= ()
+
+module HS = FStar.HyperStack
+
+#push-options "--z3rlimit 32"
+
+let rec valid_list_ext
+  (#rrel #rel: _)
+  (#k: LP.parser_kind)
+  (#t: Type)
+  (p: LP.parser k t)
+  (h1: HS.mem)
+  (sl1: LP.slice rrel rel)
+  (pos1: U32.t)
+  (pos1' : U32.t)
+  (h2: HS.mem)
+  (sl2: LP.slice rrel rel)
+  (pos2: U32.t)
+  (pos2' : U32.t)
+: Lemma
+  (requires (
+    LP.valid_list p h1 sl1 pos1 pos1' /\
+    U32.v pos2 <= U32.v pos2' /\
+    U32.v pos2' <= U32.v sl2.LP.len /\
+    LP.live_slice h2 sl2 /\
+    LP.bytes_of_slice_from_to h1 sl1 pos1 pos1' `Seq.equal` LP.bytes_of_slice_from_to h2 sl2 pos2 pos2'
+  ))
+  (ensures (
+    LP.valid_list p h1 sl1 pos1 pos1' /\
+    LP.valid_list p h2 sl2 pos2 pos2' /\
+    LP.contents_list p h1 sl1 pos1 pos1' ==
+    LP.contents_list p h2 sl2 pos2 pos2'
+  ))
+  (decreases (U32.v pos1' - U32.v pos1))
+=
+  LP.valid_list_equiv p h1 sl1 pos1 pos1' ;
+  LP.valid_list_equiv p h2 sl2 pos2 pos2' ;
+  assert (Seq.length (LP.bytes_of_slice_from_to h1 sl1 pos1 pos1') == Seq.length (LP.bytes_of_slice_from_to h2 sl2 pos2 pos2'));
+  assert (U32.v pos2' - U32.v pos2 == U32.v pos1' - U32.v pos1);
+  if pos1 = pos1'
+  then begin
+    LP.valid_list_nil p h1 sl1 pos1;
+    LP.valid_list_nil p h2 sl2 pos2
+  end else begin
+    let pos1_ = LP.get_valid_pos p h1 sl1 pos1 in
+    assert (U32.v pos1_ <= U32.v pos1');
+    LP.valid_facts p h1 sl1 pos1;
+    let pos2_ = pos2 `U32.add` (pos1_ `U32.sub` pos1) in
+    LP.parse_strong_prefix p (LP.bytes_of_slice_from h1 sl1 pos1) (LP.bytes_of_slice_from_to h1 sl1 pos1 pos1_);
+    assert (LP.bytes_of_slice_from_to h1 sl1 pos1 pos1_ `Seq.equal` Seq.slice (LP.bytes_of_slice_from_to h1 sl1 pos1 pos1') 0 (U32.v pos1_ - U32.v pos1));
+    assert (LP.bytes_of_slice_from_to h2 sl2 pos2 pos2_ `Seq.equal` Seq.slice (LP.bytes_of_slice_from_to h2 sl2 pos2 pos2') 0 (U32.v pos2_ - U32.v pos2));
+    LP.parse_strong_prefix p (LP.bytes_of_slice_from_to h1 sl1 pos1 pos1_) (LP.bytes_of_slice_from_to h2 sl2 pos2 pos2_);
+    LP.parse_strong_prefix p (LP.bytes_of_slice_from_to h2 sl2 pos2 pos2_) (LP.bytes_of_slice_from h2 sl2 pos2);
+    assert (Some? (LP.parse p (LP.bytes_of_slice_from h2 sl2 pos2)));
+    LP.valid_facts p h2 sl2 pos2;
+    assert (LP.valid p h2 sl2 pos2);
+    assert (pos2_ == LP.get_valid_pos p h2 sl2 pos2);
+    assert (LP.bytes_of_slice_from_to h1 sl1 pos1_ pos1' `Seq.equal` Seq.slice (LP.bytes_of_slice_from_to h1 sl1 pos1 pos1') (U32.v pos1_ - U32.v pos1) (U32.v pos1' - U32.v pos1));
+    assert (LP.bytes_of_slice_from_to h2 sl2 pos2_ pos2' `Seq.equal` Seq.slice (LP.bytes_of_slice_from_to h2 sl2 pos2 pos2') (U32.v pos2_ - U32.v pos2) (U32.v pos2' - U32.v pos2));
+    valid_list_ext p h1 sl1 pos1_ pos1' h2 sl2 pos2_ pos2';
+    LP.contents_list_eq p h1 sl1 pos1 pos1' ;
+    LP.valid_list_cons p h2 sl2 pos2 pos2'
+  end
+
+#pop-options
+
+let destr_list_spec
+  (#p: parser1)
+  (#inv: memory_invariant)
+  (x: lptr p inv)
+: Tot (read_repr_spec
+    (option (ptr p inv & lptr p inv))
+    True
+    (destr_list_post x)
+    (fun _ -> False)
+  )
+= fun _ ->
+  Correct (match deref_list_spec x with
+  | [] -> None
+  | a :: q ->
+    let base = x.rlptr_base in
+    let len = B.len base in
+    let sl = LP.make_slice base len in
+    let ps = get_parser p in
+    if len = 0ul
+    then LP.valid_list_nil ps inv.h0 sl 0ul;
+    LP.valid_list_cons_recip ps inv.h0 sl 0ul len;
+    let pos = LP.get_valid_pos ps inv.h0 sl 0ul in
+    let b_hd = B.gsub base 0ul pos in
+    let len_tl = len `U32.sub` pos in
+    let b_tl = B.gsub base pos len_tl in
+    let sl_hd = LP.make_slice b_hd pos in
+    let sl_tl = LP.make_slice b_tl len_tl in
+    LP.valid_facts ps inv.h0 sl 0ul;
+    LP.parse_strong_prefix ps (LP.bytes_of_slice_from inv.h0 sl 0ul) (LP.bytes_of_slice_from inv.h0 sl_hd 0ul);
+    LP.valid_facts ps inv.h0 sl_hd 0ul;
+    valid_list_ext ps inv.h0 sl pos len inv.h0 sl_tl 0ul len_tl;
+    Some (mk_ptr p inv b_hd pos, {
+      rlptr_base = b_tl;
+      rlptr_len = len_tl;
+  }))
+
+inline_for_extraction
+let destr_list_impl
+  (#p: parser1)
+  (#inv: memory_invariant)
+  (x: lptr p inv)
+: Tot (read_repr_impl
+    (option (ptr p inv & lptr p inv))
+    True
+    (destr_list_post x)
+    (fun _ -> False)
+    inv
+    (destr_list_spec x)
+  )
+= mk_read_repr_impl
+    (option (ptr p inv & lptr p inv))
+    True
+    (destr_list_post x)
+    (fun _ -> False)
+    inv
+    (destr_list_spec x)
+    (fun _ ->
+      let ps = Ghost.hide (get_parser p) in
+      let base = x.rlptr_base in
+      let len = x.rlptr_len in
+      let sl = LP.make_slice base len in
+      if x.rlptr_len = 0ul
+      then begin
+        LP.valid_list_nil ps inv.h0 sl 0ul;
+        Correct None
+      end else begin
+        LP.valid_list_cons_recip ps inv.h0 sl 0ul len;
+        let pos = (dsnd p).jumper sl 0ul in
+        let b_hd = B.sub base 0ul pos in
+        let len_tl = len `U32.sub` pos in
+        let b_tl = B.sub base pos len_tl in
+        let sl_hd = LP.make_slice b_hd pos in
+        let sl_tl = LP.make_slice b_tl len_tl in
+        LP.valid_facts ps inv.h0 sl 0ul;
+        LP.parse_strong_prefix ps (LP.bytes_of_slice_from inv.h0 sl 0ul) (LP.bytes_of_slice_from inv.h0 sl_hd 0ul);
+        LP.valid_facts ps inv.h0 sl_hd 0ul;
+        valid_list_ext ps inv.h0 sl pos len inv.h0 sl_tl 0ul len_tl;
+        Correct (Some (mk_ptr p inv b_hd pos, {
+          rlptr_base = b_tl;
+          rlptr_len = len_tl;
+        }))
+      end
+    )
+
+inline_for_extraction
+let destr_list
+  #p #inv x
+=
+  Read?.reflect (| destr_list_spec x, destr_list_impl x |)
